veric/semax_loop.v
@@ -78,6 +78,58 @@ Lemma funassert_update_tycon:
 intros; apply same_glob_funassert. rewrite glob_types_update_tycon. auto.
 Qed.
 
+
+Lemma tycontext_evolve_refl : forall Delta, tycontext_evolve Delta Delta.
+Proof.
+intros.
+split; auto.
+intros. destruct ((temp_types Delta)!id) as [[? ?]|]; auto.
+split; auto. destruct b; reflexivity.
+Qed.
+
+
+Lemma tycontext_evolve_join:
+  forall Delta Delta1 Delta2,
+   tycontext_evolve Delta Delta1 ->
+   tycontext_evolve Delta Delta2 ->
+   tycontext_evolve Delta (join_tycon Delta1 Delta2).
+Proof.
+intros [[[A B] C] D] [[[A1 B1] C1] D1] [[[A2 B2] C2] D2]
+  [? [? [? ?]]] [? [? [? ?]]];
+simpl in *;
+ repeat split; auto.
+ clear - H H3.
+intro id; specialize (H id); specialize (H3 id).
+ unfold temp_types in *; simpl in *.
+ destruct (A ! id) as [[? ?]|].
+ destruct (A1 ! id) as [[? ?]|] eqn:?; [ | contradiction].
+ destruct (A2 ! id) as [[? ?]|] eqn:?; [ | contradiction].
+ destruct H,H3; subst t1 t0.
+ rewrite (join_te_eqv _ _ _ _ _ _ Heqo Heqo0).
+ split; auto. destruct b,b0; inv H0; auto.
+ rewrite join_te_denote2.
+ unfold te_one_denote.
+ destruct (A1 ! id) as [[? ?]|]; [contradiction|].
+ auto.
+Qed.
+
+Lemma tycontext_evolve_update_tycon:
+ forall c Delta, tycontext_evolve Delta (update_tycon Delta c)
+ with tycontext_evolve_join_labeled:
+ forall l Delta, tycontext_evolve Delta (join_tycon_labeled l Delta).
+Proof.
+clear tycontext_evolve_update_tycon.
+induction c; simpl; intros; try destruct o; try apply tycontext_evolve_refl;
+try apply initialized_tycontext_evolve.
+eapply tycontext_evolve_trans; [ apply IHc1 | apply IHc2].
+apply tycontext_evolve_join; auto.
+auto.
+clear tycontext_evolve_join_labeled.
+induction l; simpl; auto; intros.
+apply tycontext_evolve_join; auto.
+Qed.
+
+
 Lemma semax_ifthenelse : 
    forall Delta P (b: expr) c d R,
       bool_type (typeof b) = true ->
@@ -124,7 +176,8 @@ eapply subp_trans'; [ | apply H3].
 apply derives_subp; apply andp_derives; auto.
 unfold exit_tycon; simpl. destruct ek; simpl; auto. 
 intros ? [? ?]; split; auto.
-apply typecheck_environ_join2; auto.
+apply typecheck_environ_join2 with Delta'; auto;
+  apply tycontext_evolve_update_tycon.
 repeat rewrite var_types_update_tycon. auto.
 repeat rewrite glob_types_update_tycon. auto.
 destruct (current_function k); destruct H0; split; auto.
